src/CSL/RefinementIdempotenceModule.v
@@ -1,0 +1,513 @@
+(* TODO: need a better name. This file is supposed to help bridge the gap from
+   the generic RefinementAdequacy.v to the layer specific versions *)
+
+From Transitions Require Import Relations Rewriting.
+
+Require Import Spec.Proc.
+Require Import Spec.ProcTheorems.
+Require Import Spec.Layer.
+Require Export CSL.WeakestPre CSL.Refinement CSL.Adequacy CSL.RefinementAdequacy CSL.ThreadReg.
+From iris.algebra Require Import auth frac agree gmap list.
+From iris.base_logic.lib Require Import invariants.
+From iris.proofmode Require Import tactics.
+Unset Implicit Arguments.
+
+Import RelationNotations.
+From Transitions Require Import Relations.
+
+Print tregG.
+SearchAbout "treg".
+
+Module Type refinement_type.
+  Context (OpC OpT: Type → Type).
+  Context (Λc: Layer OpC) (Λa: Layer OpT).
+  Context (impl: LayerImpl OpC OpT).
+  Context (Σ: gFunctors).
+  Context (exmachG : gFunctors → Type).
+  Existing Class exmachG.
+  Notation compile_op := (compile_op impl).
+  Notation compile_rec := (compile_rec impl).
+  Notation compile_seq := (compile_seq impl).
+  Notation compile := (compile impl).
+  Notation recover := (recover impl).
+  Notation compile_proc_seq := (compile_proc_seq impl).
+  Context `{CFG: cfgPreG OpT Λa Σ}.
+  Context `{INV: Adequacy.invPreG Σ}.
+  Context `{REG: inG Σ (csumR countingR (authR (optionUR (exclR unitC))))}.
+  Context {Hinstance: ∀ Σ, exmachG Σ → irisG OpC Λc Σ}.
+  Context {Hinstance_reg: ∀ Σ, exmachG Σ → tregG Σ}.
+  Context (crash_inner: forall {_ : @cfgG OpT Λa Σ} {_: exmachG Σ}, iProp Σ).
+  Context (exec_inner: forall {_ : @cfgG OpT Λa Σ} {_: exmachG Σ}, iProp Σ).
+  Context (crash_param: forall (_ : @cfgG OpT Λa Σ) (_ : exmachG Σ), Type).
+  Context (crash_inv: forall {H1 : @cfgG OpT Λa Σ} {H2 : exmachG Σ},
+              @crash_param _ H2 → iProp Σ).
+  Context (crash_starter: forall {H1 : @cfgG OpT Λa Σ} {H2 : exmachG Σ},
+              @crash_param _ H2 → iProp Σ).
+  Context (exec_inv: forall {_ : @cfgG OpT Λa Σ} {_ : exmachG Σ}, iProp Σ).
+  Context (einv_persist: forall {H1 : @cfgG OpT Λa Σ} {H2 : _},
+              Persistent (exec_inv H1 H2)).
+  Context (cinv_persist: forall {H1 : @cfgG OpT Λa Σ} {H2 : _}
+            {P: crash_param _ _}, Persistent (crash_inv H1 H2 P)).
+  (*
+  Context (init_prop: forall {_ : @cfgG OpT Λa Σ} {_: exmachG Σ}, iProp Σ).
+   *)
+
+  Context (E: coPset).
+  Context (nameIncl: nclose sourceN ⊆ E).
+  (* TODO: we should get rid of rec_seq if we're not exploiting vertical comp anymore *)
+  Context (recv: proc OpC unit).
+  Context (recsingle: recover = rec_singleton recv).
+
+  Context (register_spec: ∀ {H: exmachG Σ}, ∃ (Interp: OpState Λc → iProp Σ),
+                (∀ n σ, @state_interp _ _ _ (Hinstance _ H) (n, σ)
+                                     -∗ thread_count_interp n ∗ Interp σ) ∧
+                ∀ n σ, thread_count_interp n ∗ Interp σ -∗ state_interp (n, σ)).
+
+  Context (refinement_op_triples:
+             forall {H1 H2 T1 T2} j K `{LanguageCtx OpT T1 T2 Λa K} (op: OpT T1),
+               j ⤇ K (Call op) ∗ Registered ∗ (@exec_inv H1 H2) ⊢
+                 WP compile (Call op) {{ v, j ⤇ K (Ret v) ∗ Registered  }}).
+
+  Context (exec_inv_source_ctx: ∀ {H1 H2}, exec_inv H1 H2 ⊢ source_ctx).
+
+  (* There are types of transitions that change a "version number":
+
+     1) Recovery concludes -> Run user program
+     2) User program finishes -> Run new user program
+     3) Crash -> Run recovery
+
+     For transition 1, the layer state does not change, but we change
+     the version number for invariants and the number of registered threads.
+
+   *)
+
+  (* TODO: probably should say that this has to be given using Tej's record setter stuff *)
+  Context (set_inv_reg: exmachG Σ → invG Σ → tregG Σ → exmachG Σ).
+  Context (set_inv_reg_spec1:
+             ∀ Hex Hinv Hreg, @iris_invG _ _ _ (Hinstance _ (set_inv_reg Hex Hinv Hreg)) = Hinv).
+  Context (set_inv_reg_spec2:
+             ∀ Hex Hinv Hreg, Hinstance_reg _ (set_inv_reg Hex Hinv Hreg) = Hreg).
+  Context (set_inv_reg_spec3:
+             ∀ Hex Hinv Hreg, set_inv_reg (set_inv_reg Hex Hinv Hreg) Hinv Hreg =
+                              (set_inv_reg Hex Hinv Hreg)).
+
+  Definition post_crash {Hex: exmachG Σ} (P: ∀ {_: exmachG Σ}, iProp Σ) : iProp Σ :=
+    (∀ n σ σ' (Hcrash: Λc.(crash_step) σ (Val σ' tt)) Hinv' Hreg',
+        state_interp (n, σ) ==∗
+                     ∃ Hex', let _ := set_inv_reg Hex' Hinv' Hreg' in
+                             |={E}=> state_interp (1, σ') ∗ P)%I.
+
+  Definition post_finish {Hex: exmachG Σ} (P: ∀ {_: exmachG Σ}, iProp Σ) : iProp Σ :=
+    (∀ n σ σ' (Hcrash: Λc.(finish_step) σ (Val σ' tt)) Hinv' Hreg',
+        state_interp (n, σ) ==∗
+                     ∃ Hex', let _ := set_inv_reg Hex' Hinv' Hreg' in
+                             |={E}=> state_interp (1, σ') ∗ P)%I.
+
+  Definition post_recv {Hex: exmachG Σ} (P: ∀ {_: exmachG Σ}, iProp Σ) : iProp Σ :=
+    (∀ n σ Hinv' Hreg',
+        state_interp (n, σ) ==∗
+                     ∃ Hex', let _ := set_inv_reg Hex' Hinv' Hreg' in
+                             state_interp (1, σ) ∗ P)%I.
+
+  Context (recv_triple: ∀ {H1 H2} param,
+           (@crash_inv H1 H2 param) ∗ Registered ∗ (@crash_starter H1 H2 param) ⊢
+              WP recv @ NotStuck; ⊤
+                 {{ v, |={⊤,E}=> ∃ σ2a σ2a', source_state σ2a
+                       ∗ ⌜Λa.(crash_step) σ2a (Val σ2a' tt)⌝ ∗
+                       ∀ `{Hcfg': cfgG OpT Λa Σ},
+                       post_recv (λ H, source_ctx ∗ source_state σ2a' ==∗ |={⊤}=> exec_inner Hcfg' H)}}).
+
+  Context (init_absr: Λa.(OpState) → Λc.(OpState) → Prop).
+
+  Context (init_exec_inner: ∀ σ1a σ1c, init_absr σ1a σ1c →
+      (∀ `{Hinv: invG Σ} Hreg `{Hcfg: cfgG OpT Λa Σ},
+           |={⊤}=> ∃ (Hex': exmachG Σ), (source_ctx ∗ source_state σ1a) ={⊤}=∗
+             let _ := set_inv_reg Hex' Hinv Hreg in
+             exec_inner Hcfg _ ∗ state_interp (1, σ1c))%I).
+
+  Context (exec_inv_preserve_crash:
+      (∀ `{Hex: exmachG Σ} `{Hcfg: cfgG OpT Λa Σ},
+          exec_inv Hcfg Hex ={⊤, E}=∗ post_crash (λ H, |==> crash_inner Hcfg H))).
+
+  Context (crash_inv_preserve_crash:
+      (∀ `{Hex: exmachG Σ} `{Hcfg: cfgG OpT Λa Σ} param,
+          crash_inv Hcfg Hex param ={⊤, E}=∗ post_crash (λ H, |==> crash_inner Hcfg H))).
+
+  (* TODO: Much of this business is just to capture the fact that exec_inner/crash_inner
+     should not really mention invariants, because those old invariants are 'dead' *)
+  Context (crash_inner_inv :
+      (∀ `{Hex: exmachG Σ} `{Hcfg: cfgG OpT Λa Σ},
+          crash_inner Hcfg Hex ∗ source_ctx ={⊤}=∗
+          ∃ param, crash_inv Hcfg Hex param ∗ crash_starter Hcfg Hex param)).
+
+  Context (exec_inner_inv :
+      (∀ {Hex: exmachG Σ} `{Hcfg: cfgG OpT Λa Σ} Hinv,
+          exec_inner Hcfg Hex ∗ source_ctx ={⊤}=∗ exec_inv Hcfg (set_inv_reg Hex Hinv _))).
+
+  Context (exec_inv_preserve_finish:
+      (∀ `{Hex: exmachG Σ} `{Hcfg: cfgG OpT Λa Σ},
+          AllDone -∗ exec_inv Hcfg Hex ={⊤, E}=∗ ∃ (σ2a σ2a' : Λa.(OpState)), source_state σ2a
+          ∗ ⌜Λa.(finish_step) σ2a (Val σ2a' tt)⌝ ∗
+          ∀ `{Hcfg': cfgG OpT Λa Σ},
+          post_finish (λ H, source_ctx ∗ source_state σ2a' ==∗ |={⊤}=> exec_inner Hcfg' H))).
+
+End refinement_type.
+
+Module refinement (RT: refinement_type).
+  Import RT.
+  Existing Instances Hinstance Hinstance_reg einv_persist cinv_persist.
+
+  Import Reg_wp.
+
+  Lemma wp_spawn {H: exmachG Σ} {T} s E (e: proc _ T) Φ :
+    ▷ Registered
+      -∗ ▷ (Registered -∗ WP (let! _ <- e; Unregister)%proc @ s; ⊤ {{ _, True }})
+      -∗ ▷ ( Registered -∗ Φ tt)
+      -∗ WP Spawn e @ s; E {{ Φ }}.
+  Proof.
+    intros. edestruct (register_spec) as (?&?&?). eapply wp_spawn; eauto.
+  Qed.
+
+  Lemma wp_unregister {H: exmachG Σ} s E :
+    {{{ ▷ Registered }}} Unregister @ s; E {{{ RET tt; True }}}.
+  Proof.
+    intros. edestruct (register_spec) as (?&?&?). eapply wp_unregister; eauto.
+  Qed.
+
+  Lemma wp_wait {H: exmachG Σ} s E :
+    {{{ ▷ Registered }}} Wait @ s; E {{{ RET tt; AllDone }}}.
+  Proof.
+    intros. edestruct (register_spec) as (?&?&?). eapply wp_wait; eauto.
+  Qed.
+
+  Lemma refinement_triples:
+             forall {H1 H2 T1 T2} j K `{LanguageCtx OpT T1 T2 Λa K} (e: proc OpT T1),
+               wf_client e →
+               j ⤇ K e ∗ Registered ∗ (@exec_inv H1 H2) ⊢
+                 WP compile e {{ v, j ⤇ K (Ret v) ∗ Registered }}.
+  Proof.
+    intros ???? j K Hctx e Hwf.
+    iIntros "(Hj&Hreg&#Hinv)".
+    iAssert (⌜∃ ea: State Λa, True⌝)%I as %[? _].
+    {
+      iDestruct (exec_inv_source_ctx with "Hinv") as ((?&?)) "#Hctx".
+      eauto.
+    }
+    assert (Inhabited (State Λa)).
+    { eexists. eauto. }
+    assert (Inhabited Λa.(OpState)).
+    { eexists. destruct x; eauto. }
+    iInduction e as [] "IH" forall (j T2 K Hctx).
+    - iApply refinement_op_triples; iFrame; eauto.
+    - wp_ret. iFrame.
+    - wp_bind.
+      iApply wp_wand_l. iSplitL ""; last first.
+      * unshelve (iApply ("IH1" $! _ _ _ (fun x => K (Bind x p2)) with "[] Hj"); try iFrame).
+        { eapply Hwf. }
+        { iPureIntro. apply comp_ctx; auto. apply _. }
+      * iIntros (?) "(Hj&Hreg)".
+        iDestruct (exec_inv_source_ctx with "Hinv") as "#Hctx".
+        iMod (ghost_step_bind_ret with "Hj []") as "Hj".
+        { set_solver+. }
+        { eauto. }
+        iApply ("IH" with "[] [] Hj Hreg"); auto.
+        { iPureIntro. eapply Hwf. }
+    - iLöb as "IHloop" forall (init Hwf).
+      iDestruct (exec_inv_source_ctx with "Hinv") as "#Hctx".
+      iMod (ghost_step_loop with "Hj []") as "Hj".
+      { set_solver+. }
+      { eauto. }
+      wp_loop.
+      iApply wp_wand_l.
+      iSplitL ""; last first.
+      * rewrite /loop1. simpl.
+        unshelve (iApply ("IH" $! _ _ _ _ (fun x => K (Bind x
+                               (fun out => match out with
+                               | ContinueOutcome x => Loop body x
+                               | DoneWithOutcome r => Ret r
+                               end))) with "[] Hj Hreg")%proc).
+        { eauto. }
+        { iPureIntro. apply comp_ctx; auto. apply _. }
+      * iIntros (out) "(Hj&Hreg)".
+        destruct out.
+        ** iNext.
+           iMod (ghost_step_bind_ret with "Hj []") as "Hj".
+           { set_solver+. }
+           { eauto. }
+           iApply ("IHloop" with "[] Hj Hreg").
+           { eauto. }
+        ** iNext.
+           iMod (ghost_step_bind_ret with "Hj []") as "Hj".
+           { set_solver+. }
+           { eauto. }
+           wp_ret. iFrame.
+   - inversion Hwf.
+   - inversion Hwf.
+   - iDestruct (exec_inv_source_ctx with "Hinv") as "#Hctx".
+     iMod (ghost_step_spawn with "Hj []") as "(Hj&Hj')".
+     { set_solver+. }
+     { eauto. }
+     iDestruct "Hj'" as (j') "Hj'".
+     iApply (wp_spawn with "Hreg [Hj'] [Hj]").
+     { iNext. iIntros "Hreg'".
+       { wp_bind.
+         iApply (wp_wand with "[Hj' Hreg'] []").
+         { unshelve (iApply ("IH" $! _ _ _ (fun x => Bind x (fun _ => Unregister))
+                               with "[] Hj' Hreg'")).
+           { eauto. }
+           { iPureIntro. apply _. }
+         }
+         { iIntros (?) "(?&?)". iApply (wp_unregister with "[$]"). iIntros "!> ?". eauto. }
+       }
+     }
+     iIntros "!> ?". iFrame.
+  Qed.
+
+  Existing Instances INV CFG REG.
+
+  Transparent WeakestPre.iris_invG.
+  Lemma iris_invG_proj T H Hinv:
+      @iris_invG _ T _ (IrisG OpC _ Σ Hinv H) = Hinv.
+  Proof. auto. Qed.
+  Opaque WeakestPre.iris_invG.
+
+  Lemma Hinstance_eta Hex Hinv Hreg:
+      (Hinstance Σ (set_inv_reg Hex Hinv Hreg)) =
+      IrisG OpC _ Σ Hinv (@state_interp _ _ _ (Hinstance Σ (set_inv_reg Hex Hinv Hreg))).
+  Proof.
+    specialize (set_inv_reg_spec1 Hex Hinv Hreg).
+    destruct Hinstance => //=. rewrite iris_invG_proj => -> //.
+  Qed.
+
+  Lemma Hinstance_eta2 Hex Hinv Hreg:
+    IrisG OpC _ Σ Hinv (@state_interp _ _ _ (Hinstance Σ (set_inv_reg Hex Hinv Hreg))) =
+    Hinstance Σ (set_inv_reg (set_inv_reg Hex Hinv Hreg) Hinv
+                             (Hinstance_reg Σ (set_inv_reg Hex Hinv Hreg))).
+  Proof.
+    by rewrite -Hinstance_eta set_inv_reg_spec2 set_inv_reg_spec3.
+  Qed.
+
+  Lemma exmach_crash_refinement_seq {T} σ1c σ1a (es: proc_seq OpT T) :
+    init_absr σ1a σ1c →
+    wf_client_seq es →
+    ¬ proc_exec_seq Λa es (rec_singleton (Ret ())) (1, σ1a) Err →
+    ∀ σ2c res, proc_exec_seq Λc (compile_proc_seq es) (rec_singleton recv) (1, σ1c) (Val σ2c res) →
+    ∃ σ2a, proc_exec_seq Λa es (rec_singleton (Ret tt)) (1, σ1a) (Val σ2a res).
+  Proof.
+    rewrite /compile_proc_seq. intros Hinit Hwf_seq Hno_err σ2c0 ?.
+    unshelve (eapply wp_proc_seq_refinement_adequacy with
+                  (Λc := Λc)
+                  (φ := fun va vc _ _ => ⌜ va = vc ⌝%I)
+                  (E := E); eauto).
+    clear Hno_err.
+    iAssert (∀ invG H1 ρ,
+               |={⊤}=> ∃ Hex Hreg (HEQ:Hreg.(@treg_counter_inG Σ) = REG),
+               source_ctx' (ρ, σ1a) -∗ source_state σ1a ={⊤}=∗
+               let _ := set_inv_reg Hex invG Hreg in
+                 state_interp (1, σ1c) ∗
+                   own (treg_name Hreg) (Cinl (Count (-1))) ∗
+                   exec_inner H1 (set_inv_reg Hex invG Hreg))%I
+      as "Hpre".
+    {
+      iIntros (???).
+      iMod (own_alloc (Cinl (Count 0))) as (tR) "Ht".
+      { constructor. }
+      set (Hreg' := {| treg_name := tR; treg_counter_inG := _ |}).
+      iAssert (own tR (Cinl (Count 1)) ∗ own tR (Cinl (Count (-1))))%I with "[Ht]" as "(Ht&Hreg)".
+      { rewrite /Registered -own_op Cinl_op counting_op' //=. }
+      iMod (init_exec_inner $! _ _ _) as (Hex') "H"; eauto.
+      iModIntro. unshelve (iExists Hex', Hreg', _); first by eauto.
+      iIntros "#Hctx Hstate".
+      iMod ("H" with "[Hstate]") as "(Hexec&Hstate)".
+      { iFrame. iExists _; eauto. }
+      by iFrame.
+    }
+
+  clear Hinit.
+  iInduction es as [|es] "IH" forall (σ1a σ1c) "Hpre"; first by eauto.
+  - iSplit; first by (eauto using nameIncl).
+    iExists (fun cfgG (s: State Λc) => ∀ (s': State Λc)
+                  (Hcrash: Λc.(crash_step) (snd s) (Val (snd s') tt)) Hinv',
+                 |==> ∃ (Hex : exmachG Σ) (HEQ:(@Hinstance_reg _ Hex).(@treg_counter_inG Σ) = REG),
+                 let Hex' := set_inv_reg Hex Hinv' (@Hinstance_reg _ Hex) in
+                 |={E}=> state_interp (1, snd s') ∗
+                 own (treg_name _) (Cinl (Count 0)) ∗ crash_inner cfgG Hex')%I; auto.
+  iIntros (invG0 Hcfg0).
+  iMod ("Hpre" $! invG0 _ _) as (hEx Hreg HEQ) "H".
+  iExists (@state_interp _ _ _ ((Hinstance Σ (set_inv_reg hEx invG0 Hreg)))). iModIntro.
+  iIntros "(#Hsrc&Hpt0&Hstate)".
+  iMod ("H" with "Hsrc Hstate") as "(Hinterp&Hreg&Hinv)".
+  iMod (@exec_inner_inv with "[Hinv]") as "#Hinv".
+  { iSplitR ""; last by (iExists _; iFrame). iFrame. }
+  iFrame.
+  iSplitL "Hpt0 Hreg".
+  {  iPoseProof (@wp_mono with "[Hpt0 Hreg]") as "H"; swap 1 2.
+     {
+       iApply @refinement_triples. destruct (Hwf_seq) as (?&?). eauto. iFrame. iFrame "Hinv".
+       rewrite ?set_inv_reg_spec2.
+       rewrite /Registered. rewrite HEQ. auto.
+     }
+     { reflexivity. }
+     simpl. rewrite /compile_whole.
+     iModIntro.
+     iApply @wp_bind_proc_subst_weak.
+     rewrite Hinstance_eta2.
+     iApply (@wp_wand with "H [Hinv]").
+     iIntros (v) "(Hpt0&Hreg)". iFrame.
+     iApply @wp_bind_proc_subst_weak.
+     iApply (@wp_wand with "[Hreg Hpt0] []"); last first.
+     { iIntros (?) "H". iApply "H". }
+     iApply (@wp_wait with "[$]").
+     iIntros "!> Hdone".
+     iApply @wp_ret.
+     iFrame. iExists _. iFrame. iIntros (σ2c) "Hmach".
+     iPoseProof (exec_inv_preserve_finish with "Hdone Hinv") as "Hpose".
+     rewrite -Hinstance_eta2.
+     iMod "Hpose" as (σ2a σ2a') "(H&Hfina&Hfinish)".
+     iDestruct "Hfina" as %Hfina.
+     iModIntro. iExists _; iFrame; auto.
+     simpl.
+     rewrite -/wp_proc_seq_refinement.
+     iIntros (σ2c'). iIntros.
+     unshelve (iExists σ2a', _); [eauto |]; [].
+     iApply "IH".
+     { iPureIntro. destruct Hwf_seq. eauto. }
+     { iIntros.
+       destruct σ2c as (n&σ2c).
+       iMod (own_alloc (Cinl (Count 0))) as (tR_fresh') "Ht".
+       { constructor. }
+       iAssert (own tR_fresh' (Cinl (Count 1))
+                    ∗ own tR_fresh' (Cinl (Count (-1))))%I with "[Ht]" as "(Ht&Hreg)".
+       { rewrite /Registered -own_op Cinl_op counting_op' //=. }
+       set (tR''' := {| treg_name := tR_fresh'; treg_counter_inG := _ |}).
+       iSpecialize ("Hfinish" $! _ _ _ with "[] [Hmach]").
+       { eauto. }
+       { simpl. iFrame.
+         rewrite set_inv_reg_spec2.
+         rewrite set_inv_reg_spec3.
+         eauto.
+       }
+       iMod "Hfinish" as (Hex') "H".
+       iModIntro. iExists _. iExists tR'''. unshelve (iExists _); first by eauto.
+       iIntros "#Hctx' Hsrc'".
+       iMod (fupd_mask_mono with "H") as "(H&Hfinish)"; first by set_solver.
+       iFrame. iMod ("Hfinish" with "[Hsrc']") as "Hfinish".
+       {
+         iFrame "Hsrc'". iExists _. rewrite set_inv_reg_spec1. iFrame "Hctx'".
+       }
+       rewrite set_inv_reg_spec1.
+       iFrame.
+     }
+  }
+  iModIntro.
+  iSplit.
+  { iIntros (σ2c) "Hmach".
+    iPoseProof (exec_inv_preserve_crash with "Hinv") as "Hinv_post".
+    rewrite -Hinstance_eta2.
+    iMod "Hinv_post" as "Hinv_post".
+    iMod (own_alloc (Cinl (Count 0))) as (tR_fresh') "Ht".
+    { constructor. }
+    set (tR''' := {| treg_name := tR_fresh'; treg_counter_inG := _ |}).
+    iModIntro. iIntros.
+    destruct σ2c as (?&σ2c).
+    iSpecialize ("Hinv_post" $! _ _ _ Hcrash Hinv' with "[Hmach]").
+    { rewrite set_inv_reg_spec2 set_inv_reg_spec3. eauto. }
+    iMod ("Hinv_post") as (?) "H".
+    iModIntro. unshelve (iExists (set_inv_reg H Hinv' tR'''), _).
+    { rewrite set_inv_reg_spec2. eauto. }
+    rewrite ?set_inv_reg_spec2 ?set_inv_reg_spec1 ?set_inv_reg_spec3.
+    iMod ("H") as "(H&>H')".
+    iFrame.
+    eauto.
+  }
+  iClear "Hsrc".
+  iModIntro. iIntros (invG Hcfg' (?&s) (n'&s') Hcrash) "(Hinv0&#Hsrc)".
+  destruct Hcrash as ([]&(?&?)&Hputs&Hcrash).
+  inversion Hputs.
+  subst.
+  inversion Hcrash. subst.
+  inversion H. subst.
+  unshelve (iMod ("Hinv0" $! (1, s') _ _) as "Hinv0"); [ eauto | |].
+  eauto.
+  clear HEQ.
+  iDestruct "Hinv0" as (HexmachG' HEQ) "H".
+  iMod (fupd_mask_mono with "H") as "(H&Hfinish)"; first by set_solver.
+  iExists (@state_interp _ _ _ (@Hinstance Σ (set_inv_reg HexmachG' invG (Hinstance_reg Σ HexmachG')))).
+  iDestruct "Hfinish" as "(Hreg&Hcrash_inner)".
+  iPoseProof (@crash_inner_inv ((set_inv_reg HexmachG' invG (Hinstance_reg Σ HexmachG'))) _ with "[Hcrash_inner]") as "Hcrash".
+  { simpl. iFrame. iExists _. rewrite set_inv_reg_spec1. eauto. }
+  rewrite set_inv_reg_spec1.
+  iClear "Hinv".
+  iMod "Hcrash" as (param) "(#Hinv&Hstarter)".
+  iModIntro.
+  iFrame.
+  iAssert (own ((Hinstance_reg Σ HexmachG').(treg_name)) (Cinl (Count 1)) ∗
+           own ((Hinstance_reg Σ HexmachG').(treg_name)) (Cinl (Count (-1))))%I
+    with "[Hreg]" as "(Ht&Hreg)".
+  { rewrite set_inv_reg_spec2. rewrite /Registered -own_op Cinl_op counting_op' //=. }
+  iSplitL "Hstarter Hinv Hreg".
+  {
+    iPoseProof (@wp_mono with "[Hinv Hreg Hstarter IH]") as "H"; swap 1 2.
+    { iApply recv_triple. iFrame "Hstarter". iFrame. iFrame "Hinv".
+      rewrite/ Registered. rewrite set_inv_reg_spec2 HEQ.
+      eauto.
+    }
+    { reflexivity. }
+    iApply (@wp_wand with "[H] [IH]").
+    { rewrite Hinstance_eta. iApply "H". }
+    iIntros (_) "H". iIntros (σ2c) "Hinterp".
+    iMod "H". iModIntro.
+    iDestruct "H" as (σ2a σ2a') "(Hsource&Hinner&Hfinish)".
+    iExists (1, σ2a), (1, σ2a'). iFrame.
+     rewrite -/wp_proc_seq_refinement.
+     iDestruct "Hinner" as %?.
+     iSplitL "".
+     { iPureIntro. exists tt, (1, σ2a); split; eauto. econstructor. split; eauto. eauto.
+       econstructor; eauto.
+     }
+     iApply "IH".
+     { destruct Hwf_seq. eauto. }
+     { iIntros.
+       iMod (own_alloc (Cinl (Count 0))) as (tR_fresh'') "Ht".
+       { constructor. }
+       iAssert (own tR_fresh'' (Cinl (Count 1))
+                    ∗ own tR_fresh'' (Cinl (Count (-1))))%I with "[Ht]" as "(Ht&Hreg)".
+       { rewrite /Registered -own_op Cinl_op counting_op' //=. }
+       set (tR'''' := {| treg_name := tR_fresh''; treg_counter_inG := _ |}).
+       destruct σ2c.
+       iMod ("Hfinish" $! H2 _ with "Hinterp") as (Hex') "(Hinterp&Hfinish)".
+       unshelve (iExists _, _, _); first by auto.
+       iFrame.
+       iModIntro. simpl.
+       iClear "Hsrc".
+       iIntros "#Hsrc Hstate".
+       iMod ("Hfinish" with "[Hstate]") as "Hfinish".
+       { iFrame. iExists _. rewrite set_inv_reg_spec1. eauto. }
+       rewrite set_inv_reg_spec1.
+       iApply "Hfinish".
+     }
+  }
+  {
+    iIntros (σ2c) "Hmach".
+    iPoseProof (@crash_inv_preserve_crash with "Hinv") as "Hinv_post".
+    rewrite set_inv_reg_spec1.
+    iMod ("Hinv_post") as "Hinv_post".
+    iMod (own_alloc (Cinl (Count 0))) as (tR_fresh'') "Ht'".
+    { constructor. }
+    set (tR'''' := {| treg_name := tR_fresh''; treg_counter_inG := _ |}).
+    iModIntro. iIntros.
+    destruct σ2c as (?&σ2c).
+    iSpecialize ("Hinv_post" with "[] [Hmach]").
+    { iPureIntro. eauto. }
+    { eauto. }
+    iMod ("Hinv_post") as (?) "H".
+    iModIntro. unshelve (iExists (set_inv_reg _ Hinv' tR''''), _).
+    { rewrite set_inv_reg_spec2. eauto. }
+    rewrite ?set_inv_reg_spec2 ?set_inv_reg_spec1 ?set_inv_reg_spec3.
+    iMod ("H") as "(H&>H')".
+    iFrame.
+    eauto.
+  }
+  Qed.
+
+End refinement.
