src/Examples/ExMach/Adequacy.v
@@ -1,5 +1,5 @@
 From iris.algebra Require Import auth gmap frac agree.
-Require Export CSL.WeakestPre CSL.Lifting CSL.Adequacy CSL.RefinementAdequacy.
+Require Export CSL.WeakestPre CSL.Lifting CSL.Adequacy CSL.RefinementAdequacy CSL.RefinementIdempotenceModule.
 From iris.algebra Require Export functions.
 From iris.base_logic.lib Require Export invariants gen_heap.
 From iris.proofmode Require Export tactics.
